ocaml/coq_driver/test/tzel_wots.mli
@@ -7,6 +7,10 @@ val hash5 : felt -> felt -> felt -> felt -> felt -> felt
 
 val commit : felt -> felt -> felt -> felt -> felt -> felt
 
+val hash_nf : felt -> felt -> felt
+
+val nullifier : felt -> felt -> felt -> felt
+
 val pack_adrs_chain : int -> int -> int -> felt
 
 val xmss_chain_step : felt -> felt -> int -> int -> int -> felt
